Main.lean
@@ -1,5 +1,11 @@
 import Specs
 import Init.System.IO
 
+def genSpecBook : IO Unit := sorry
+
+def genRustTests : IO Unit := sorry
+
 def main : IO Unit :=
-  return
+  do
+    genSpecBook
+    genRustTests
