Specs/syntax.lean
@@ -1,5 +1,7 @@
 import Specs.abstraction.Book
 import Specs.syntax.Ast
+import Specs.syntax.EntityRoute
+import Specs.syntax.EntityKind
 import Specs.syntax.Opr
 import Specs.syntax.Text
 import Specs.syntax.Token
